{"nbformat":4,"nbformat_minor":0,"metadata":{"colab":{"provenance":[],"authorship_tag":"ABX9TyNJkOm5GCZg6qEdRqaF9D+K"},"kernelspec":{"name":"python3","display_name":"Python 3"},"language_info":{"name":"python"}},"cells":[{"cell_type":"markdown","source":["1.Find the value of T(2) for the recurrence relation T(n) = 3T(n-1) + 12n, given that T(0)=5."],"metadata":{"id":"jjxq_4hmj233"}},{"cell_type":"markdown","source":["\n","\n","### Step 1: Calculate \\( T(1) \\)\n","Using the recurrence relation for \\( n = 1 \\):\n","\n","\\[\n","T(1) = 3T(0) + 12 \\times 1\n","\\]\n","\\[\n","T(1) = 3 \\times 5 + 12 = 15 + 12 = 27\n","\\]\n","\n","### Step 2: Calculate \\( T(2) \\)\n","Now, using the recurrence relation for \\( n = 2 \\):\n","\n","\\[\n","T(2) = 3T(1) + 12 \\times 2\n","\\]\n","\\[\n","T(2) = 3 \\times 27 + 24 = 81 + 24 = 105\n","\\]\n","\n","### Final Answer:\n","\\[\n","T(2) = 105\n","\\]"],"metadata":{"id":"Khq1gBqfkEoM"}},{"cell_type":"markdown","source":["2. Given a recurrence relation, solve it using the substitution method:\n","a. T(n) = T(n-1) + c\n","b. T(n) = 2T(n/2) + n\n","c. T(n) = 2T(n/2) + c\n","d. T(n) = T(n/2) + c"],"metadata":{"id":"s5N0GeVykGT-"}},{"cell_type":"markdown","source":["Let's solve each of the given recurrence relations using the **substitution method**:\n","\n","### a. \\( T(n) = T(n-1) + c \\)\n","\n","We want to find the pattern by unrolling the recurrence:\n","\n","- Start with \\( T(n) = T(n-1) + c \\).\n","- Substitute \\( T(n-1) \\) using the recurrence:\n","  \\[\n","  T(n) = (T(n-2) + c) + c = T(n-2) + 2c\n","  \\]\n","- Substitute \\( T(n-2) \\):\n","  \\[\n","  T(n) = T(n-3) + 3c\n","  \\]\n","- Continuing this process, after \\( k \\) steps, we get:\n","  \\[\n","  T(n) = T(n-k) + kc\n","  \\]\n","- Eventually, when \\( k = n \\), \\( T(0) \\) will be the base case. Assuming \\( T(0) = T_0 \\), we have:\n","  \\[\n","  T(n) = T_0 + nc\n","  \\]\n","\n","Thus, the solution to the recurrence is:\n","\\[\n","T(n) = T_0 + nc\n","\\]\n","\n","### b. \\( T(n) = 2T(n/2) + n \\)\n","\n","We can solve this recurrence by unrolling:\n","\n","- Start with \\( T(n) = 2T(n/2) + n \\).\n","- Substitute \\( T(n/2) \\) using the recurrence:\n","  \\[\n","  T(n) = 2(2T(n/4) + n/2) + n = 4T(n/4) + n + n = 4T(n/4) + 2n\n","  \\]\n","- Substitute \\( T(n/4) \\):\n","  \\[\n","  T(n) = 4(2T(n/8) + n/4) + 2n = 8T(n/8) + n + 2n = 8T(n/8) + 3n\n","  \\]\n","- Continuing this process, after \\( k \\) steps, we get:\n","  \\[\n","  T(n) = 2^k T(n / 2^k) + kn\n","  \\]\n","- Eventually, \\( n / 2^k = 1 \\), which happens when \\( k = \\log_2 n \\). At this point, we reach the base case \\( T(1) \\), which is a constant. Let \\( T(1) = T_1 \\), so:\n","  \\[\n","  T(n) = 2^{\\log_2 n} T(1) + n \\log_2 n\n","  \\]\n","  Simplifying \\( 2^{\\log_2 n} = n \\), we get:\n","  \\[\n","  T(n) = n T_1 + n \\log_2 n\n","  \\]\n","  \n","Thus, the solution is:\n","\\[\n","T(n) = O(n \\log n)\n","\\]\n","\n","### c. \\( T(n) = 2T(n/2) + c \\)\n","\n","This recurrence is similar to part (b), but with a constant \\( c \\) instead of \\( n \\). Let's unroll it:\n","\n","- Start with \\( T(n) = 2T(n/2) + c \\).\n","- Substitute \\( T(n/2) \\):\n","  \\[\n","  T(n) = 2(2T(n/4) + c) + c = 4T(n/4) + 2c + c = 4T(n/4) + 3c\n","  \\]\n","- Substitute \\( T(n/4) \\):\n","  \\[\n","  T(n) = 4(2T(n/8) + c) + 3c = 8T(n/8) + 4c + 3c = 8T(n/8) + 7c\n","  \\]\n","- Continuing this process, after \\( k \\) steps, we get:\n","  \\[\n","  T(n) = 2^k T(n / 2^k) + (2^k - 1)c\n","  \\]\n","- Eventually, when \\( k = \\log_2 n \\), \\( n / 2^k = 1 \\), so we get:\n","  \\[\n","  T(n) = n T(1) + (n - 1)c\n","  \\]\n","  Assuming the base case is constant, say \\( T(1) = T_1 \\), the solution is:\n","  \\[\n","  T(n) = O(n)\n","  \\]\n","\n","### d. \\( T(n) = T(n/2) + c \\)\n","\n","Let's solve this recurrence using substitution:\n","\n","- Start with \\( T(n) = T(n/2) + c \\).\n","- Substitute \\( T(n/2) \\):\n","  \\[\n","  T(n) = (T(n/4) + c) + c = T(n/4) + 2c\n","  \\]\n","- Substitute \\( T(n/4) \\):\n","  \\[\n","  T(n) = T(n/8) + 3c\n","  \\]\n","- Continuing this process, after \\( k \\) steps, we get:\n","  \\[\n","  T(n) = T(n / 2^k) + kc\n","  \\]\n","- Eventually, when \\( k = \\log_2 n \\), \\( n / 2^k = 1 \\), so we get:\n","  \\[\n","  T(n) = T(1) + c \\log_2 n\n","  \\]\n","  Assuming \\( T(1) = T_1 \\), the solution is:\n","  \\[\n","  T(n) = O(\\log n)\n","  \\]\n","\n","### Summary of Solutions:\n","\n","1. \\( T(n) = T(n-1) + c \\) → \\( T(n) = T_0 + nc \\)\n","2. \\( T(n) = 2T(n/2) + n \\) → \\( T(n) = O(n \\log n) \\)\n","3. \\( T(n) = 2T(n/2) + c \\) → \\( T(n) = O(n) \\)\n","4. \\( T(n) = T(n/2) + c \\) → \\( T(n) = O(\\log n) \\)"],"metadata":{"id":"z7kWIGAekaSZ"}},{"cell_type":"markdown","source":["3. Given a recurrence relation, solve it using the recursive tree approach:\n","a. T(n) = 2T(n-1) +1\n","b. T(n) = 2T(n/2) + n"],"metadata":{"id":"tNw41vtHkdCY"}},{"cell_type":"markdown","source":["### Solving Recurrence Relations Using the Recursive Tree Approach\n","\n","Let's break down both recurrence relations using the **recursive tree approach**, which helps visualize the work done at each level of recursion and the total cost.\n","\n","### a. \\( T(n) = 2T(n-1) + 1 \\)\n","\n","#### Step 1: Unroll the recurrence\n","\n","To understand how the function behaves at each step, let's unroll the recurrence:\n","\n","- \\( T(n) = 2T(n-1) + 1 \\)\n","- \\( T(n-1) = 2T(n-2) + 1 \\)\n","- \\( T(n-2) = 2T(n-3) + 1 \\)\n","- ...\n","- \\( T(1) = 2T(0) + 1 \\)\n","\n","#### Step 2: Visualizing the recursive tree\n","\n","At the top of the tree (level 0), we have \\( T(n) = 2T(n-1) + 1 \\). The work done at this level is 1 (constant). Then, at level 1, we have two calls, each contributing \\( T(n-1) \\), and each of those performs 1 unit of work. At level 2, we have four calls to \\( T(n-2) \\), each doing 1 unit of work. The process continues down until we reach the base case \\( T(0) \\), which is assumed to be a constant.\n","\n","#### Step 3: Tree structure\n","\n","- At level 0: 1 call to \\( T(n) \\), performing 1 unit of work.\n","- At level 1: 2 calls to \\( T(n-1) \\), each performing 1 unit of work.\n","- At level 2: 4 calls to \\( T(n-2) \\), each performing 1 unit of work.\n","- At level 3: 8 calls to \\( T(n-3) \\), each performing 1 unit of work.\n","- ...\n","- At level \\( k \\): \\( 2^k \\) calls to \\( T(n-k) \\), each performing 1 unit of work.\n","\n","#### Step 4: Total work\n","\n","The total work is the sum of the work done at each level. The number of levels is \\( n \\) (since the argument decreases by 1 each time). The work done at each level is \\( 2^k \\) (where \\( k \\) is the level number), and the total work is:\n","\n","\\[\n","W(n) = 1 + 2 + 4 + 8 + \\dots + 2^{n-1}\n","\\]\n","\n","This is a geometric series, and its sum is:\n","\n","\\[\n","W(n) = 2^n - 1\n","\\]\n","\n","Thus, the total work done is \\( O(2^n) \\).\n","\n","#### Final Answer:\n","\\[\n","T(n) = O(2^n)\n","\\]\n","\n","---\n","\n","### b. \\( T(n) = 2T(n/2) + n \\)\n","\n","#### Step 1: Unroll the recurrence\n","\n","Let's unroll the recurrence to understand the work done at each level:\n","\n","- \\( T(n) = 2T(n/2) + n \\)\n","- \\( T(n/2) = 2T(n/4) + n/2 \\)\n","- \\( T(n/4) = 2T(n/8) + n/4 \\)\n","- ...\n","\n","#### Step 2: Visualizing the recursive tree\n","\n","At the top level (level 0), we have \\( T(n) = 2T(n/2) + n \\), and it performs \\( n \\) work. Then, at level 1, we have two calls to \\( T(n/2) \\), each performing \\( n/2 \\) work, for a total of \\( n \\) work at that level. At level 2, we have four calls to \\( T(n/4) \\), each performing \\( n/4 \\) work, again totaling \\( n \\) work at that level. The process continues down until we reach the base case.\n","\n","#### Step 3: Tree structure\n","\n","- At level 0: 1 call to \\( T(n) \\), performing \\( n \\) units of work.\n","- At level 1: 2 calls to \\( T(n/2) \\), each performing \\( n/2 \\) units of work, so total work at this level is \\( n \\).\n","- At level 2: 4 calls to \\( T(n/4) \\), each performing \\( n/4 \\) units of work, so total work at this level is \\( n \\).\n","- At level 3: 8 calls to \\( T(n/8) \\), each performing \\( n/8 \\) units of work, so total work at this level is \\( n \\).\n","- ...\n","- At level \\( k \\): \\( 2^k \\) calls to \\( T(n / 2^k) \\), each performing \\( n / 2^k \\) work, so total work at this level is \\( n \\).\n","\n","#### Step 4: Total work\n","\n","The total work at each level is \\( n \\), and there are \\( \\log_2 n \\) levels (because at each level, the problem size halves). So the total work is:\n","\n","\\[\n","W(n) = n \\times \\log_2 n\n","\\]\n","\n","Thus, the total work done is \\( O(n \\log n) \\).\n","\n","#### Final Answer:\n","\\[\n","T(n) = O(n \\log n)\n","\\]\n","\n","---\n","\n","### Summary of Results:\n","\n","1. \\( T(n) = 2T(n-1) + 1 \\) → \\( T(n) = O(2^n) \\)\n","2. \\( T(n) = 2T(n/2) + n \\) → \\( T(n) = O(n \\log n) \\)"],"metadata":{"id":"jm48H-g2kjkf"}},{"cell_type":"markdown","source":[],"metadata":{"id":"BbDZSuavk0x2"}}]}